coq/proof/SoundReduceMaydiff.v
@@ -15,6 +15,7 @@ Require Import paco.
 Import Opsem.
 
 Require Import TODO.
+Require Import Postcond.
 Require Import Validator.
 Require Import GenericValues.
 Require Import SimulationLocal.
@@ -25,7 +26,7 @@ Require Import SoundBase.
 Set Implicit Arguments.
 
 
-Lemma reduce_maydiff_sound
+Lemma reduce_maydiff_lessdef_sound
       m_src m_tgt
       conf_src st_src
       conf_tgt st_tgt
@@ -34,7 +35,40 @@ Lemma reduce_maydiff_sound
       (STATE: InvState.Rel.sem conf_src conf_tgt st_src st_tgt invst invmem inv)
       (MEM: InvMem.Rel.sem conf_src conf_tgt st_src.(Mem) st_tgt.(Mem) invmem):
   <<STATE: InvState.Rel.sem conf_src conf_tgt st_src st_tgt invst invmem
-                            (Postcond.reduce_maydiff inv)>> /\
+                            (reduce_maydiff_lessdef inv)>> /\
   <<MEM: InvMem.Rel.sem conf_src conf_tgt st_src.(Mem) st_tgt.(Mem) invmem>>.
 Proof.
 Admitted.
+
+Lemma reduce_maydiff_non_physical_sound
+      m_src m_tgt
+      conf_src st_src
+      conf_tgt st_tgt
+      invst0 invmem inv
+      (CONF: valid_conf m_src m_tgt conf_src conf_tgt)
+      (STATE: InvState.Rel.sem conf_src conf_tgt st_src st_tgt invst0 invmem inv)
+      (MEM: InvMem.Rel.sem conf_src conf_tgt st_src.(Mem) st_tgt.(Mem) invmem):
+  exists invst1,
+    <<STATE: InvState.Rel.sem conf_src conf_tgt st_src st_tgt invst1 invmem
+                              (reduce_maydiff_non_physical inv)>> /\
+    <<MEM: InvMem.Rel.sem conf_src conf_tgt st_src.(Mem) st_tgt.(Mem) invmem>>.
+Proof.
+Admitted.
+
+Lemma reduce_maydiff_sound
+      m_src m_tgt
+      conf_src st_src
+      conf_tgt st_tgt
+      invst0 invmem inv
+      (CONF: valid_conf m_src m_tgt conf_src conf_tgt)
+      (STATE: InvState.Rel.sem conf_src conf_tgt st_src st_tgt invst0 invmem inv)
+      (MEM: InvMem.Rel.sem conf_src conf_tgt st_src.(Mem) st_tgt.(Mem) invmem):
+  exists invst1,
+    <<STATE: InvState.Rel.sem conf_src conf_tgt st_src st_tgt invst1 invmem
+                              (reduce_maydiff inv)>> /\
+    <<MEM: InvMem.Rel.sem conf_src conf_tgt st_src.(Mem) st_tgt.(Mem) invmem>>.
+Proof.
+  unfold reduce_maydiff.
+  exploit reduce_maydiff_lessdef_sound; eauto. i. des.
+  exploit reduce_maydiff_non_physical_sound; eauto.
+Qed.
